execution/examples/BoardroomVotingTest.v
@@ -28,7 +28,7 @@ Definition modulus : Z := 201697267445741585806196628073.
 Definition generator : Z := 3.
 
 Axiom modulus_prime : prime modulus.
-Instance axioms : BoardroomAxioms Z := BigZp.boardroom_axioms modulus modulus_prime.
+Instance axioms : BoardroomAxioms Z := boardroom_axioms_Z modulus modulus_prime.
 
 Lemma generator_nonzero : generator !== 0.
 Proof. discriminate. Qed.
@@ -50,8 +50,7 @@ Definition votes_for : nat := 4.
 Definition sk n := (Z.of_nat n + 1234583932) * (modulus - 23241)^159338231.
 
 (* Make a list of secret keys, here starting at i=7 *)
-Definition sks : list Z :=
-  Eval native_compute in map sk (seq 7 num_parties).
+Definition sks : list Z := map sk (seq 7 num_parties).
 
 (* Make a list of votes for each party *)
 Definition svs : list bool :=
@@ -62,16 +61,17 @@ Definition svs : list bool :=
 
 (* Compute the public keys for each party *)
 Definition pks : list Z :=
-  Eval native_compute in map compute_public_key sks.
+  Eval vm_compute in map compute_public_key sks.
 
 Definition rks : list Z :=
-  Eval native_compute in map (reconstructed_key pks) (seq 0 (length pks)).
+  Eval vm_compute in map (reconstructed_key pks) (seq 0 (length pks)).
 
 (* In this example we just use xor for the hash function, which is
    obviously not cryptographically secure. *)
 Definition hash_func (l : list positive) : positive :=
   N.succ_pos (fold_right (fun p a => N.lxor (Npos p) a) 1%N l).
 
+  
 Definition AddrSize := (2^128)%N.
 Instance Base : ChainBase := LocalChainBase AddrSize.
 Instance ChainBuilder : ChainBuilderType := LocalChainBuilderDepthFirst AddrSize.
@@ -92,7 +92,7 @@ Module BV := BoardroomVoting Params. Import BV.
 (* Compute the signup messages that would be sent by each party.
    We just use the public key as the chosen randomness here. *)
 Definition signups : list Msg :=
-  Eval native_compute in map (fun '(sk, pk, i) => make_signup_msg sk 5 i)
+  Eval vm_compute in map (fun '(sk, pk, i) => make_signup_msg sk 5 i)
                              (zip (zip sks pks) (seq 0 (length sks))).
 
 (* Compute the submit_vote messages that would be sent by each party *)
@@ -100,7 +100,7 @@ Definition signups : list Msg :=
    using the make_vote_msg function provided by the contract.
    In this example we just use the secret key as the random parameters. *)
 Definition votes : list Msg :=
-  Eval native_compute in map (fun '(i, sk, sv, rk) => make_vote_msg pks i sk sv sk sk sk)
+  Eval vm_compute in map (fun '(i, sk, sv, rk) => make_vote_msg pks i sk sv sk sk sk)
                              (zip (zip (zip (seq 0 (length pks)) sks) svs) rks).
 
 Definition A a :=
@@ -121,7 +121,7 @@ Proof.
   exact tm.
 Defined.
 
-Definition voters_map : AddrMap unit := FMap.of_list (map (fun a => (a, tt)) addrs).
+Definition voters_map : AddrMap unit := AddressMap.of_list (map (fun a => (a, tt)) addrs).
 
 
 Definition deploy_setup :=
@@ -146,7 +146,7 @@ Definition boardroom_example : option nat :=
   do chain <- add_block chain [];
   let dep := build_act creator (create_deployment 0 boardroom_voting deploy_setup) in
   do chain <- add_block chain [dep];
-  do caddr <- hd_error (FMap.keys (lc_contracts (lcb_lc chain)));
+  do caddr <- hd_error (AddressMap.keys (lc_contracts (lcb_lc chain)));
   let send addr m := build_act addr (act_call caddr 0 (serialize m)) in
   let calls := map (fun '(addr, m) => send addr m) (zip addrs signups) in
   do chain <- add_block chain calls;
